arithmetic/coq/Verif_add_with_carry.v
@@ -5,45 +5,110 @@ Require Import Didactica.arithmetic.
 Require Import Didactica.Add.
 Require Import Didactica.number.
 
-Lemma body_add_with_carry : semax_body Vprog Gprog f_add_with_carry add_with_carry_spec.
+Lemma overflowing_add : forall a b : Z,
+  digit_bound a ->
+  digit_bound b ->
+  (and
+    (digit_bound (Z.modulo
+      (Z.add a b)
+      Int64.modulus))
+    (eq
+      (Int64.repr (Z.add a b))
+      (Int64.repr (Z.modulo
+        (Z.add a b)
+        Int64.modulus)))).
+Proof.
+  intros. split.
+  - unfold digit_bound in *.
+    assert
+      (0 <= (a + b) mod Int64.modulus < Int64.modulus)
+    by apply
+      (Z.mod_pos_bound
+        (a + b)
+        Int64.modulus
+        ltac:(rep_lia)).
+    rep_lia.
+  - Search (eq (Int64.repr _) (Int64.repr _)).
+    apply Int64.eqm_samerepr. unfold Int64.eqm.
+    unfold Zbits.eqmod. exists ((a + b)/Int64.modulus).
+    rewrite (Z.mul_comm ((a + b)/Int64.modulus) Int64.modulus).
+    apply Z_div_mod_eq_full.
+Qed.
+
+Lemma ltu_translation : forall a b,
+  digit_bound a ->
+  digit_bound b ->
+  (eq 
+    (Int64.ltu
+      (Int64.repr a)
+      (Int64.repr b))
+    (Z.ltb a b)).
+Proof.
+Admitted.
+
+Lemma bool_bound : forall b,
+  0 <= (Z.b2z b) <= 1.
+Proof.
+Admitted.
+
+Lemma body_add_with_carry :
+  (semax_body Vprog Gprog f_add_with_carry add_with_carry_spec).
 Proof.
   start_function.
-  unfold digit_bound in *.
+  generalize
+    (add_back_to_bool
+      Int64.modulus
+      carry_in
+      left_digit
+      right_digit);
+  intros back_to_bool; simpl in back_to_bool.
   forward. deadvars!. normalize.
-(*
-  replace
-    (Int64.repr (left_digit + Z.b2z carry_in))
-  with
-    (Int64.repr
-      (Z.modulo
-        (left_digit + Z.b2z carry_in)
-        Int64.max_unsigned)).
-  admit.
-  Search (@eq int _ _).
-  Check eq.
-
-  unfold Int64.repr.
-  replace
-    (Int64.Z_mod_modulus
-      ((left_digit + Z.b2z carry_in) mod Int64.max_unsigned))
-  with
-    (((left_digit + Z.b2z carry_in) mod Int64.max_unsigned) mod Int64.max_unsigned).
-  reflexiv
-  rewrite Int64.Z_mod_modulus_eq.
-  Search Int64.Z_mod_modulus.
-
-  Search Int64.repr.
+  generalize
+    (bool_bound carry_in);
+  intros carry_bound.
+  generalize
+    (overflowing_add
+      (Z.b2z carry_in)
+      left_digit
+      ltac:(unfold digit_bound; rep_lia)
+      H);
+  intros [temporary_bound overflowed];
+  rewrite overflowed; clear overflowed.
+  remember
+    ((Z.b2z carry_in + left_digit) mod Int64.modulus)
+  as temporary.
   forward. normalize.
-  forward.
-  replace
-    (Int64.ltu
-      (Int64.repr (left_digit + Z.b2z carry_in))
-      (Int64.repr (Z.b2z carry_in)))
-  with
-    (Z.ltb
-      (Z.modulo (Z.b2z carry_in + left_digit) Int64.max_unsigned)
-      (Z.b2z carry_in)). admit.
+  generalize
+    (overflowing_add
+      temporary
+      right_digit
+      temporary_bound
+      H0);
+  intros [result_bound overflowed];
+  rewrite overflowed; clear overflowed.
+  remember
+    ((temporary + right_digit) mod Int64.modulus)
+  as result.
+  forward. normalize.
+  rewrite
+    (ltu_translation
+      temporary
+      (Z.b2z carry_in)
+      temporary_bound
+      ltac:(unfold digit_bound; rep_lia)).
+  rewrite
+    (ltu_translation
+      result
+      right_digit
+      result_bound
+      H0).
+  generalize
+    (bool_bound (Z.ltb temporary (Z.b2z carry_in)));
+  intros left_overflow_bound.
+  generalize
+    (bool_bound (Z.ltb result right_digit));
+  intros right_overflow_bound.
   normalize.
-  entailer!. forward.
-  *)
-Admitted.
+  rewrite back_to_bool.
+  forward.
+Qed.
